fix rsa implementation

code/experimental/rsa/MGF.fst
@@ -12,8 +12,12 @@ open Lib
 module U32 = FStar.UInt32
 module U8 = FStar.UInt8
 
+#set-options "--lax"
+
+(* SHA 256 *)
+let hLen = 32ul
 val hash_sha256:
-	mHash:lbytes 32ul ->
+	mHash:lbytes hLen ->
 	len:U32.t ->
 	m:uint8_p{length m = U32.v len /\ disjoint mHash m} -> Stack unit
 	(requires (fun h -> live h m /\ live h mHash))
@@ -22,12 +26,12 @@ val hash_sha256:
 		 
 let hash_sha256 mHash len m = SHA2_256.hash mHash m len
 
-type mgf_state (accLen:blen) = lbytes U32.(32ul +^ 4ul +^ 4ul +^ 32ul +^ accLen)
+type mgf_state (accLen:blen) = lbytes U32.(hLen +^ 4ul +^ 4ul +^ hLen +^ accLen)
 
-let get_mgfseed_counter #a (st:mgf_state a) : lbytes U32.(32ul +^ 4ul) = Buffer.sub st 0ul U32.(32ul +^ 4ul)
-let get_counter #a (st:mgf_state a) : lbytes 4ul = Buffer.sub st U32.(32ul +^ 4ul) 4ul 
-let get_mHash #a (st:mgf_state a) : lbytes 32ul = Buffer.sub st U32.(32ul +^ 4ul +^ 4ul) 32ul
-let get_acc #a (st:mgf_state a) : lbytes a = Buffer.sub st U32.(32ul +^ 4ul +^ 4ul +^ 32ul) a
+let get_mgfseed_counter #a (st:mgf_state a) : lbytes U32.(hLen +^ 4ul) = Buffer.sub st 0ul U32.(hLen +^ 4ul)
+let get_counter #a (st:mgf_state a) : lbytes 4ul = Buffer.sub st U32.(hLen +^ 4ul) 4ul 
+let get_mHash #a (st:mgf_state a) : lbytes hLen = Buffer.sub st U32.(hLen +^ 4ul +^ 4ul) hLen
+let get_acc #a (st:mgf_state a) : lbytes a = Buffer.sub st U32.(hLen +^ 4ul +^ 4ul +^ hLen) a
 
 let mgf_state_inv a (st:mgf_state a) = 
            let mgfseed_counter = get_mgfseed_counter st in
@@ -50,8 +54,8 @@ let mgf_state_st_inv (aLen:blen) (st:mgf_state aLen) (h:FStar.HyperStack.mem) =
 
 val mgf_loop:
 	count_max:U32.t ->
-	mgfseed:lbytes 32ul ->
-	accLen:blen{U32.v accLen = 32 * (U32.v count_max)} -> 
+	mgfseed:lbytes hLen ->
+	accLen:blen{U32.v accLen = (U32.v hLen) * (U32.v count_max)} -> 
 	st:mgf_state accLen{disjoint st mgfseed} ->
 	counter:U32.t{U32.v counter <= U32.v count_max} -> Stack unit
 	(requires (fun h -> live h mgfseed /\ mgf_state_st_inv accLen st h ))
@@ -59,7 +63,7 @@ val mgf_loop:
 			live h1 mgfseed /\ mgf_state_st_inv accLen st h1 /\
 			modifies_1 st h0 h1))
 
-#set-options "--z3rlimit 150 --max_fuel 2"
+#reset-options "--z3rlimit 300 --max_fuel 2"
 
 let rec mgf_loop count_max mgfseed accLen st counter =
 	if U32.(counter <^ count_max) then begin
@@ -69,41 +73,41 @@ let rec mgf_loop count_max mgfseed accLen st counter =
 		let acc = get_acc st in
 		
 		(**) assert(length c = 4);
-		(**) assert(length mgfseed_counter = 32 + 4);
 		c.(0ul) <- uint32_to_uint8 (U32.(counter >>^ 24ul));
 		c.(1ul) <- uint32_to_uint8 (U32.(counter >>^ 16ul));
 		c.(2ul) <- uint32_to_uint8 (U32.(counter >>^ 8ul));
 		c.(3ul) <- uint32_to_uint8 counter;
 		
 		(* blit mgfseed 0ul tmp 0ul 32ul; *)
-		blit c 0ul mgfseed_counter 32ul 4ul;
-		hash_sha256 mHash U32.(32ul +^ 4ul) mgfseed_counter;
-		(**) assert(length mHash = 32);
-		(**) assert(32 * (U32.v counter) < length acc);
-		blit mHash 0ul acc U32.(32ul *^ counter) 32ul;
+		(**) assert(length mgfseed_counter = U32.v hLen + 4);
+		blit c 0ul mgfseed_counter hLen 4ul;
+		(**) assert(length mHash = U32.v hLen);
+		hash_sha256 mHash U32.(hLen +^ 4ul) mgfseed_counter;
+		(**) assert((U32.v hLen) * (U32.v counter) < length acc);
+		(**) assert((U32.v hLen) * (U32.v counter) + U32.v hLen <= length acc);
+		blit mHash 0ul acc U32.(hLen *^ counter) hLen;
 		mgf_loop count_max mgfseed accLen st U32.(counter +^ 1ul) end
 
-
 val mgf_sha256:
-	mgfseed:lbytes 32ul ->
+	mgfseed:lbytes hLen ->
 	len:blen -> res:lbytes len{disjoint mgfseed res} -> Stack unit
 	(requires (fun h -> live h res /\ live h mgfseed))
 	(ensures (fun h0 _ h1 ->
 		live h0 res /\ live h0 mgfseed /\
 		live h1 res /\ live h1 mgfseed /\ modifies_1 res h0 h1))
 
-#set-options "--z3rlimit 50"
+#reset-options "--z3rlimit 50"
 
 let mgf_sha256 mgfseed len res =
 	push_frame();
-	let count_max = U32.((len -^ 1ul) /^ 32ul +^ 1ul) in
-	(**) assume(32 * (U32.v count_max) > 0 /\ 32 * (U32.v count_max) <= 65536);
-	let accLen: blen  = U32.(32ul *^ count_max) in
-	(**) assume(32 + 4 + 4 + 32 + U32.v accLen > 0 /\ 32 + 4 + 4 + 32 + U32.v accLen <= 65536);
-	let stLen = U32.(32ul +^ 4ul +^ 4ul +^ 32ul +^ accLen) in
+	let count_max = U32.((len -^ 1ul) /^ hLen +^ 1ul) in
+	(**) assume(0 < (U32.v hLen) * (U32.v count_max) /\ (U32.v hLen) * (U32.v count_max) <= 65536);
+	let accLen: blen  = U32.(hLen *^ count_max) in
+	(**) assume(U32.v hLen + 4 + 4 + U32.v hLen + U32.v accLen > 0 /\ U32.v hLen + 4 + 4 + U32.v hLen + U32.v accLen <= 65536);
+	let stLen = U32.(hLen +^ 4ul +^ 4ul +^ hLen +^ accLen) in
 	let st: mgf_state accLen = create 0uy stLen in
 	let mgfseed_counter = get_mgfseed_counter st in
-	blit mgfseed 0ul mgfseed_counter 0ul 32ul;
+	blit mgfseed 0ul mgfseed_counter 0ul hLen;
 	mgf_loop count_max mgfseed accLen st 0ul;
 	let acc = get_acc st in
 	blit acc 0ul res 0ul len;
